nueva ver actions

Practica7/Actions2.v
@@ -31,27 +31,20 @@ Definition differ_at_most_memory (s s': State) (ma: madd) : Prop :=
   (* Action preconditions *)
   Definition Pre (s : State) (a : Action) : Prop :=
     match a with
-    | read va => (ctxt_vadd_accessible ctxt) va = true 
-                  -> (aos_activity s) = running 
-                   -> exists (ma : madd), 
-                      (va_mapped_to_ma s va ma 
-                        -> match memory s ma with
-                            | Some page => is_RW (page_content page)
-                            | _ => False
-                           end)
-    | write va val => (ctxt_vadd_accessible ctxt) va = true 
-                        -> (aos_activity s) = running 
-                         -> exists (ma : madd), 
-                            (va_mapped_to_ma s va ma 
-                              -> match memory s ma with
-                                  | Some page => is_RW (page_content page)
-                                  | _ => False
-                                 end)
-    | chmod => (aos_activity s) = waiting -> 
-                  match ((oss s) (active_os s)) with 
-                  | Some os => hcall os = None
-                  | _ => False
-                  end
+    | read va => (ctxt_vadd_accessible ctxt) va = true
+                      /\ (aos_activity s) = running
+                      /\ exists (ma : madd) (pg : page),
+                          (va_mapped_to_ma s va ma
+                          /\ memory s ma = Some pg
+                          /\ is_RW (page_content pg))
+    | write va val => (ctxt_vadd_accessible ctxt) va = true
+                      /\ (aos_activity s) = running
+                      /\ exists (ma : madd) (pg : page),
+                          (va_mapped_to_ma s va ma
+                          /\ memory s ma = Some pg
+                          /\ is_RW (page_content pg))
+    | chmod => (aos_activity s) = waiting
+               /\ (exists (o : os), oss s (active_os s) = Some o /\ hcall o = None)
     end.
 
 Definition differ_in_state (s s': State) (em : exec_mode) (act : os_activity) :=
@@ -66,29 +59,28 @@ Definition differ_in_state (s s': State) (em : exec_mode) (act : os_activity) :=
   Definition Post (s : State) (a : Action) (s' : State) : Prop :=
     match a with
     | read va => s = s'
-    | write va val => exists (ma : madd), (va_mapped_to_ma s va ma 
-                                          -> (memory s') = 
+    | write va val => exists (ma : madd), va_mapped_to_ma s va ma 
+                                          /\ (memory s') = 
                                               update (memory s) ma
-                                                 (mk_page (RW (Some val)) 
-                                                        (Os (active_os s)))
-                                           ) -> differ_at_most_memory s s' ma
-    | chmod => (trusted_os ctxt s -> 
-                 differ_in_state s s' svc running)
-               \/ 
-               (~(trusted_os ctxt s) -> 
-                differ_in_state s s' usr running)
+                                                (mk_page (RW (Some val)) (Os (active_os s)))
+                                          /\ differ_at_most_memory s s' ma
+    | chmod => (trusted_os ctxt s /\ differ_in_state s s' svc running)
+               \/
+               (~(trusted_os ctxt s) /\ differ_in_state s s' usr running)
     end.
 
 (* if the hypervisor (hypervisor running si activity es waiting)
  or a trusted OS is running 
 the processor must be in supervisor mode*)
-  Definition valid_state_iii (s : State) : Prop :=  
+  Definition valid_state_iii (s : State) : Prop :=
   ((aos_activity s) = waiting) \/
-    ((aos_activity s) = running -> trusted_os ctxt s) 
+    ((aos_activity s) = running /\ trusted_os ctxt s)
   -> (aos_exec_mode s) = svc.
-  
+
   Definition inyective {A B : Set} (pmap : A ⇸ B) :=
     forall x y, pmap x = pmap y -> x = y.
+
+(*
 
 (* paged_owned_by ((memory s) ((hypervisor s) (active_os s) phyadd)) = (active_os s) *)
   Definition valid_state_v_aux (s : State) : Prop :=
@@ -148,8 +140,32 @@ pages owned by the hypervisor *)
      | _ => True (* si no hay match quiero que sea vdd *)
     end.
 
+*)
+
+Definition Prop5 (s : State) : Prop :=
+  forall (pa : padd) (pm : padd -> option madd) (ma : madd) (pg : page),
+      (hypervisor s) (active_os s) = Some pm
+      /\ pm pa = Some ma
+      /\ memory s ma = Some pg
+      /\ page_owned_by pg = Os (active_os s)
+      /\ inyective pm.
+
+Definition Prop6 (s : State) : Prop :=
+  forall (pg pg' : page) (vtm : vadd -> option madd) (va : vadd) (ma : madd) (o : os_ident),
+    page_content pg = PT vtm 
+    /\ page_owned_by pg = Os o
+    /\ vtm va = Some ma
+    /\ memory s ma = Some pg'
+    /\ (ctxt_vadd_accessible ctxt va = true -> page_owned_by pg' = Os o)
+    /\ (ctxt_vadd_accessible ctxt va = false -> page_owned_by pg' = Hyp).
+
+Definition valid_state (s : State) : Prop :=
+    valid_state_iii s /\ Prop5 s /\ Prop6 s.
+
+(*
   Definition valid_state (s : State) : Prop :=
     valid_state_iii s /\ valid_state_v s /\ valid_state_vi s.
+*)
 
   Inductive one_step : State -> Action -> State -> Prop :=
   | step : forall (s s': State) (a: Action), 
@@ -158,71 +174,90 @@ pages owned by the hypervisor *)
   Notation "a ⇒ s ↪ s'" := (one_step s a s') (at level 50).
 
 
+
   Theorem one_step_preserves_prop_iii : forall (s s' : State) (a : Action),
       a ⇒ s ↪ s' -> valid_state_iii s'.
   Proof.
   intros.
-  destruct H.
-  induction a.
-  - simpl in H1.
-    rewrite H1 in H.
-    unfold valid_state in H.
-    elim H. intros.
-    exact H2.
-  - unfold valid_state_iii.
-    intros.
-    destruct H1.
-    unfold Pre in H0.
-    admit.
-  - case_eq (aos_activity s); intros.
-    unfold valid_state in H. elim H. intros.
-    unfold valid_state_iii in H3.
-    + simpl in H1.
-      unfold valid_state_iii. intros.
-      elim H3.
-        -- intros.
-      admit. (*
-      elim H1.
-      * unfold valid_state_iii. intros.
-        unfold valid_state in H. elim H. intros.
-        unfold valid_state_iii in H5.
-        unfold differ_in_state in H3.
-        elim H5.
-      *)
-    + unfold valid_state in H. elim H. intros.
-      unfold valid_state_iii in H3.
-
-
-
-    elim H1; intros.
-    + unfold valid_state_iii.
-      intros.
-      unfold differ_in_state in H2.
-      elim H2. intros.
-    + elim H2; intros.
-      exact H3.
+  inversion H.
+  inversion H0.
+  unfold valid_state_iii. intros.
+  destruct a.
+  - inversion H2.
+    rewrite H9 in H6.
+    elim H6; intros.
+    + reflexivity.
+    + exact H8.
+  - inversion H2.
+    elim H9. intros.
+    elim H11. intros.
+    unfold differ_at_most_memory in H13.
+    elim H13. intros. elim H15. intros. elim H17. intros.
+    rewrite <- H16.
+    apply H6.
+    elim H8; intros.
+    + left.
+      rewrite H18.
+      exact H20.
+    + right.
+      elim H20. intros.
+      split.
+      rewrite H18.
+      exact H21.
       unfold trusted_os.
-      
-  unfold valid_state_iii.
-      admit.
-    + elim H2; intros.
-      
-
-
- simpl in H0.
-  induction a; induction H.
-  induction H.
-  
-
+      rewrite H14.
+      exact H22.
+  - inversion H2.
+    + elim H9. intros.
+      unfold differ_in_state in H11.
+      elim H11. intros.
+      exact H12.
+    + elim H9. intros.
+      unfold differ_in_state in H11.
+      elim H11. intros. elim H13. intros. elim H15. intros.
+      elim H8; intros.
+      * absurd (aos_activity s' = waiting).
+        rewrite H14. discriminate.
+        exact H18.
+      * unfold trusted_os in H10.
+        rewrite H16 in H10.
+        elim H18. intros.
+        absurd (trusted_os ctxt s').
+        exact H10.
+        exact H20.
   Qed.
 
 
-  Theorem read_isolation : forall (s s' : State) (va : vadd), read va ⇒ s ↪ s -> 
-  exists ma: madd, va_mapped_to_ma s va ma /\ exists pg: page, Some pg = (memory s) ma /\ (page_owned_by pg) = Os (active_os s).
+  Theorem read_isolation : forall (s s' : State) (va : vadd), read va ⇒ s ↪ s' -> 
+  exists ma: madd, va_mapped_to_ma s va ma /\ 
+  exists pg: page, Some pg = (memory s) ma /\ (page_owned_by pg) = Os (active_os s).
   Proof.
   intros.
-  destruct H.
+  inversion H.
+  unfold valid_state in H0. elim H0. intros. elim H7. intros.
+  inversion H2.
+  unfold Pre in H1.
+  elim H1. intros. elim H12. intros. elim H14. intros. elim H15. intros.
+  exists x.
+  split.
+  - rewrite <- H10.
+    elim H16. intros.
+    exact H17.
+  - destruct (memory s x).
+    + exists p.
+      rewrite H10 in H8.
+      elim (H8 (curr_page ) (hypervisor_map (active_os s')) x p).
+    + contradiction H15.
   Qed.
+
+Definition Prop5 (s : State) : Prop :=
+  forall (pa : padd) (pm : padd -> option madd) (ma : madd) (pg : page),
+      (hypervisor s) (active_os s) = Some pm
+      /\ pm pa = Some ma
+      /\ memory s ma = Some pg
+      /\ page_owned_by pg = Os (active_os s)
+      /\ inyective pm.
+
 
 End Actions.
 
